InputStream adaptors

TestModels/dafny-dependencies/StandardLibrary/runtimes/java/src/main/java/Streams/InputStreamAsDataStream.java
@@ -1,0 +1,39 @@
+package Streams;
+
+import StandardLibrary_Compile.Streams_Compile.DataStream;
+import Std_Compile.BulkActions_Compile.Batched;
+import Std_Compile.Producers_Compile.Producer;
+import Std_Compile.Wrappers_Compile.Option;
+
+import java.io.InputStream;
+import java.math.BigInteger;
+
+public class InputStreamAsDataStream implements DataStream<Exception> {
+
+    private final InputStream inputStream;
+    private boolean read = false;
+
+    public InputStreamAsDataStream(InputStream inputStream) {
+        this.inputStream = inputStream;
+    }
+
+    @Override
+    public Option<BigInteger> ContentLength() {
+        return Option.create_None(null);
+    }
+
+    @Override
+    public boolean Replayable() {
+        return false;
+    }
+
+    @Override
+    public Producer<Batched<Byte, Exception>> Reader() {
+        if (read) {
+            throw new IllegalStateException("Already read");
+        }
+        read = true;
+
+        return new InputStreamAsProducer(inputStream);
+    }
+}
