TestModels/dafny-dependencies/StandardLibrary/runtimes/java/src/main/java/Streams/InputStreamAsProducer.java
@@ -1,0 +1,97 @@
+package Streams;
+
+import Std_Compile.BulkActions_Compile.BatchArrayWriter;
+import Std_Compile.BulkActions_Compile.BatchReader;
+import Std_Compile.BulkActions_Compile.Batched;
+import Std_Compile.Consumers_Compile.Consumer;
+import Std_Compile.Consumers_Compile.IConsumer;
+import Std_Compile.Producers_Compile.Producer;
+import Std_Compile.Producers_Compile._Companion_Producer;
+import Std_Compile.Producers_Compile.__default;
+import Std_Compile.Wrappers_Compile.Option;
+import dafny.Array;
+import dafny.DafnySequence;
+import dafny.Tuple0;
+import dafny.TypeDescriptor;
+
+import java.io.IOException;
+import java.io.InputStream;
+import java.math.BigInteger;
+
+public class InputStreamAsProducer implements Producer<Batched<Byte, Exception>> {
+
+    private final InputStream inputStream;
+    private long totalRead;
+
+    private static final TypeDescriptor<Byte> T_TD = TypeDescriptor.BYTE;
+    private static final TypeDescriptor<Exception> E_TD = TypeDescriptor.reference(Exception.class);
+    private static final TypeDescriptor<Batched<Byte, Exception>> BATCHED_TD =
+            Batched._typeDescriptor(T_TD, E_TD);
+
+    public InputStreamAsProducer(InputStream inputStream) {
+        this.inputStream = inputStream;
+        this.totalRead = 0;
+    }
+
+    @Override
+    public BigInteger ProducedCount() {
+        return BigInteger.valueOf(totalRead);
+    }
+
+    @Override
+    public Option<BigInteger> Remaining() {
+        return Option.create_None(TypeDescriptor.BIG_INTEGER);
+    }
+
+    @Override
+    public Option<Batched<Byte, Exception>> Next() {
+        try {
+            int value = inputStream.read();
+            if (value == -1) {
+                // TODO: EOI
+                return Option.create_None(BATCHED_TD);
+            } else {
+                Batched batched = Batched.create_BatchValue(T_TD, E_TD, (byte)value);
+                return Option.create_Some(BATCHED_TD, batched);
+            }
+        } catch (IOException e) {
+            return Option.create_Some(null, Batched.create_BatchError(T_TD, E_TD, e));
+        }
+    }
+
+    @Override
+    public void ForEach(IConsumer<Batched<Byte, Exception>> consumer) {
+        __default.DefaultForEach(BATCHED_TD, this, consumer);
+    }
+
+    @Override
+    public Option<Batched<Byte, Exception>> Fill(Consumer<Batched<Byte, Exception>> consumer) {
+        if (consumer instanceof BatchArrayWriter) {
+            BatchArrayWriter<Byte, Exception> writer = (BatchArrayWriter) consumer;
+            int n = writer.Capacity().dtor_value().intValueExact();
+            byte[] buffer = new byte[n];
+            try {
+                int count = inputStream.read(buffer, 0, n);
+                if (count == -1) {
+                    consumer.Accept(Batched.create_EndOfInput(T_TD, E_TD));
+                } else {
+                    totalRead += count;
+                    Array<Byte> dafnyArray = Array.wrap(buffer);
+                    BatchReader<Byte, Exception> reader = new BatchReader(T_TD, E_TD);
+                    reader.__ctor(DafnySequence.fromArrayRange(T_TD, dafnyArray, 0, count));
+                    reader.Fill(consumer);
+                }
+            } catch (IOException e) {
+                writer.Accept(Batched.create_BatchError(T_TD, E_TD, e));
+            }
+            return Option.create_None(BATCHED_TD);
+        }
+
+        return __default.DefaultFill(BATCHED_TD, this, consumer);
+    }
+
+    @Override
+    public Option<Batched<Byte, Exception>> Invoke(Tuple0 tuple0) {
+        return _Companion_Producer.Next(null, this);
+    }
+}
